src/ASN1/ASN1.Spec.Choice.fst
@@ -80,7 +80,7 @@ let make_gen_choice_parser
 
 let make_asn1_choice_parser
   (lc : list (asn1_id_t * asn1_content_k) {Cons? lc})
-  (pf : ((Cons? lc) /\ List.noRepeats (List.map fst lc)))
+  (pf : squash ((Cons? lc) /\ List.noRepeats (List.map fst lc)))
   (#s : _)
   (k : asn1_k s)
   (lp : list (asn1_id_t & gen_parser) {Cons? lp})
@@ -92,7 +92,7 @@ let make_asn1_choice_parser
 
 let make_asn1_choice_parser_twin
   (lc : list (asn1_id_t * asn1_content_k) {Cons? lc})
-  (pf : ((Cons? lc) /\ List.noRepeats (List.map fst lc)))
+  (pf : squash ((Cons? lc) /\ List.noRepeats (List.map fst lc)))
   (#s : _)
   (k : asn1_k s)
   (lp : list (asn1_id_t & gen_parser) {Cons? lp})
@@ -105,7 +105,7 @@ let make_asn1_choice_parser_twin
 
 let make_asn1_choice_parser_twin_cases_injective
   (lc : list (asn1_id_t * asn1_content_k) {Cons? lc})
-  (pf : ((Cons? lc) /\ List.noRepeats (List.map fst lc)))
+  (pf : squash ((Cons? lc) /\ List.noRepeats (List.map fst lc)))
   (#s : _)
   (k : asn1_k s)
   (lp : list (asn1_id_t & gen_parser) {Cons? lp})
